src/compiler/Generator_dynamic.thy
@@ -74,7 +74,7 @@ imports Printer
            "Abstract_associationclass" "Associationclass"
            "Context"
            (* OCL (added) *)
-           "End" "Instance" "BaseType" "State" "Transition"
+           "End" "Instance" "BaseType" "State" "Transition" "Tree"
 
            (* Isabelle syntax *)
            "generation_syntax"
@@ -1334,13 +1334,16 @@ structure USE_parse = struct
 
   (* *)
 
+  fun natural0 s = case Int.fromString s of SOME i => From.nat i
+                                          | NONE => Scan.fail "Syntax error"
+
+  val natural = Parse.number >> natural0
+
   val unlimited_natural =  ident_star >> (fn "*" => META.Mult_star
                                            | "\<infinity>" => META.Mult_infinity
                                            | _ => Scan.fail "Syntax error")
-                        || Parse.number >> (fn s => META.Mult_nat
-                                                      (case Int.fromString s of
-                                                         SOME i => From.nat i
-                                                       | NONE => Scan.fail "Syntax error"))
+                        || Parse.number >> (META.Mult_nat o natural0)
+
   val term_base =
        Parse.number >> (META.OclDefInteger o From.string)
     || Parse.float_number >> (META.OclDefReal o (From.pair From.string From.string o
@@ -1767,6 +1770,19 @@ val () =
         , META.OclDefPP ( From.option From.binding n
                        , mk_pp_state thy s_pre
                        , From.option (mk_pp_state thy) s_post)))
+end
+\<close>
+
+subsection\<open>Setup of Meta Commands for OCL: Tree\<close>
+
+ML\<open>
+local
+  open USE_parse
+in
+val () =
+  outer_syntax_command @{mk_string} @{command_keyword Tree} ""
+    (natural -- natural)
+    (fn (n_w, n_h) => K (META.META_class_tree (META.OclClassTree (n_w, n_h))))
 end
 (*val _ = print_depth 100*)
 \<close>
